Picinae_amd64.v
@@ -47,6 +47,11 @@ Open Scope N.
 Inductive x64var :=
   (* Main memory: *)
   | V_MEM64
+  (* Instruction Pointer Register, read and written by Ghidra, but does not
+     represent the location of the current instruction.  We model it to
+     reduce our TCB in that we don't handle its translation specially in
+     the lifter. *)
+  | R_RIP
   (* Flags (1-bit registers): *)
   | R_AF | R_CF | R_DF | R_OF | R_PF | R_SF | R_ZF
   (* Segment selectors (16-bit registers): *)
@@ -78,6 +83,7 @@ Inductive x64var :=
 Definition x64typctx v :=
   match v with
   | V_MEM64 => Some (8*2^64)
+  | R_RIP => Some 64
   | R_AF | R_CF | R_DF | R_OF | R_PF | R_SF | R_ZF => Some 1
   | R_CS | R_DS | R_ES | R_FS | R_GS | R_SS => Some 16
   | R_FPU_CONTROL => Some 16
