tutorial/BasicLoops.v
@@ -1,0 +1,613 @@
+(** #<link rel="stylesheet" href="sf.css"># *)
+(** * Basic Loops *)
+
+(* ################################################################# *)
+(** * Introduction *)
+
+(** This chapter goes deeper into the structure and meaning of Proofs
+    and covers examples of more complicated programs with loops. We'll
+    also be using a more sophisticated toy architecture but we'll delay
+    its exposition and covering the theoretical and implementation
+    underpinnings of Picinae to a later chapter. *)
+
+(* ################################################################# *)
+(** * Setting It Up *)
+
+Require Export Picinae_core.
+Require Export Picinae_theory.
+Require Export Picinae_statics.
+Require Export Picinae_finterp.
+Require Export Picinae_simplifier_v1_1.
+Require Import Picinae_pilbox32.
+Require Import NArith.
+Require Import Structures.Equalities.
+Require Import Lia ZifyN.
+Require Import Utf8.
+Import PIL32Notations.
+Open Scope N.
+Ltac fail_seek ::= idtac.
+
+
+(* ================================================================= *)
+(** ** The AddLoop Program *)
+
+(** Our first example program computes the sum of two numbers by repeatedly
+    incrementing one register and decrementing the other until the latter
+    is zero.  Again we use a toy architecture and handcrafted IL code.
+    The toy architecture we choose this time is specified as a 32 bits
+    architecture.  This is a descriptive, not prescriptive, categorization(?)
+    of the architecture.  We typically call an architecture X-bits if its
+    largest memory range uses X-bit addresses and most of its working
+    registers are X-bits.
+
+    At the end of this chapter we'll look at example programs lifted directly
+    from real world code. *)
+Module Addloop.
+
+Module Addloop1.
+Definition addloop (s:store) (a:addr) : option (N * stmt) :=
+  match a with
+    (* nop *)
+  | 100 => Some(4, Nop)
+    (* :addloop *)
+    (* beqz r1 :done *)
+  | 104 => Some(4, If (BinOp OP_EQ (Var R_R1) (Word 0 32)) (Jmp (Word 120 32)) (Nop))
+    (* sub r1 0x1 *)
+  | 108 => Some(4, Move R_R1 (BinOp OP_MINUS (Var R_R1) (Word 1 32)))
+    (* add r2 0x1 *)
+  | 112 => Some(4, Move R_R2 (BinOp OP_PLUS (Var R_R2) (Word 1 32)))
+    (* jmp :addloop *)
+  | 116 => Some(4, Jmp (Word 104 32))
+    (* :done *)
+    (* mov r2 r0 *)
+  | 120 => Some(4, Move R_R0 (Var R_R2))
+  | _ => None
+  end.
+
+(** As before we define our Initial trace condition, our Invariants, and exits
+    in a dedicated section so they can refer to common variables. *)
+
+Section Invs.
+
+  Variable s:store.
+  Variable r1 r2:N.
+  Definition Entry t xs' := startof t xs' = (Addr 100, s).
+  Definition Models := models pil32typctx s.
+  Definition TraceConditions s' := s' R_R1 = r1 /\ s' R_R2 = r2.
+  Definition Init t xs' := Entry t xs' /\ Models /\ TraceConditions s.
+
+(** Our postcondition is where we start to see the first signs of the intrinsic trickiness
+    in reasoning about behavior at the machine code level.  This program doesn't simply
+    sum two numbers.  It sums them _modulo 32_.  This introduces difficulties both in
+    mentally reasoning about proofs as well as constructing proofs.  At this level it is
+    a common phenomenon to find yourself looking at a simple equation and wondering "wait,
+    is this actually even true?" Later we'll show off _psimpl_, our automated modular
+    arithmetic simplifier that can handle a large class of modular and bit arithmetic
+    expressions. *)
+  Definition postcondition n := n = (r1 + r2) mod 2 ^ 32.
+
+(** This is a control flow graph (CFG) of the addloop program showing which instructions
+    execute after which other instructions.  It shows that the instruction at address 100
+    always falls through to the instruction at 104, the instruction at 104 may fall through to
+    108 or branch to 120, the instruction at 116 always jumps to 104, and all other instructions
+    fall through similarly to 100:
+
+<<
+             100
+              |
+       +---> 104 ------+
+       :      |        :
+       :     108       :
+       :      |        :
+       :     112       :
+       :      |        :
+       +---- 116       :
+                       :
+             120 <-----+
+              |
+             124
+>>
+
+    The type of proofs we're exploring say "For all traces that match some starting criteria
+    (Init) and a given set of invariants and exit points (Invs and exit) all executions of
+    the program
+
+        1. reach an invariant or exit
+        2. whenever they reach an invariant the invariant is satisfied and execution continues
+           and reaches an invariant or exit."
+
+    Picinae accomplishes the "reaches an invariant or exit" guarantee by creating a proof obligation
+    at every non-exit invariant and requiring abstract execution to continue until an exit or invariant
+    (possibly the same one) is encountered.  This is the function of the `destruct_invs XX.` tactic
+    in our proofs.
+
+    Specifically, if we place invariants at addresses 100, 104, and 124, and an exit at 124 then
+    Picinae will produce 2 subgoals we need to prove - one from address 100 and the other from 104.
+    This decomposes the proof into 2 paths of execution:
+
+<<
+              100
+               |
+              104              +---> 104 ------+
+                               :      |        :
+                               :      |        :
+                               :      |        :
+                               :      |        :
+                               :      |        :
+                               +----- +        :
+                                               :
+                                      + <------+
+                                      |
+                                     124
+>>
+
+    It accomplishes the "invariant is satisfied" guarantee by 1) populating the
+    hypothesis space with the proposition of the invariant from which we're starting
+    execution and 2) dropping the proof into an ordinary Coq proof whenever
+    it reaches the invariant. It replaces the goal with the specified invariant,
+    which will often depend on the result of abstract execution. *)
+
+
+  Definition Invs1 (t:trace) :=
+    match t with (Addr a, s)::_ =>
+      match a with
+      | 100 => Some (TraceConditions s)
+      | 104 => Some (((s R_R1) + (s R_R2)) mod 2 ^ 32 = (r1 + r2) mod 2 ^ 32)
+      | 124 => Some (postcondition (s R_R0))
+      | _ => None
+      end
+    | _ => None
+    end.
+
+Definition addloop_exit (t:trace) :=
+  match t with (Addr a,_)::_ =>
+    match a with
+      124 => true
+    | _   => false
+    end
+  | _ => false
+  end.
+
+End Invs.
+
+Theorem addloop_welltyped : welltyped_prog pil32typctx addloop.
+Proof. Picinae_typecheck. Qed.
+
+Theorem addloop_partial_correctness:
+  forall s t xs' r1 r2
+    (INIT: Init s r1 r2 t xs'),
+    satisfies_all addloop (Invs1 r1 r2) addloop_exit (xs'::t).
+Proof.
+  Local Ltac step := pil32_step.
+
+  intros s t xs' r1 r2 (ENTRY & MDL & R1 & R2).
+  apply prove_invs.
+
+  (* Base Case *)
+  simpl. rewrite ENTRY. step. split; assumption.
+
+  (* Inductive Case *)
+  (* Explain the current proof obligation *)
+  intros.
+  unfold Entry in *; erewrite startof_prefix in ENTRY; try eassumption.
+  eapply models_at_invariant; try eassumption. apply addloop_welltyped. intro MDL1.
+  clear - PRE MDL1. rename t1 into t; rename s1 into s.
+  destruct_inv 32 PRE.
+
+  (* 100 -> 104 *)
+  destruct PRE as (R1 & R2).
+  step.
+  subst. reflexivity.
+
+  (* 104 -> 104 / 120 *)
+  rename PRE into INV. step.
+
+  (* 104 -> 120 *)
+  step.
+
+  rewrite N.eqb_eq in BC. rewrite BC in *. elimstore.
+      rewrite N.add_0_l in INV. rewrite <-INV; clear INV.
+      rewrite N.mod_small; lia.
+
+  (* 104 -> 104 *)
+  step. step. step.
+  rewrite INV. reflexivity.
+
+Qed.
+End Addloop1.
+
+(** What happens if we don't include an invariant anywhere in the loop?
+
+    Considering replacing this with a simpler example that uses nops and an
+    unconditional branch. *)
+
+Module AddloopAndBeyond.
+Section Invs.
+  Variable s:store.
+  Variable r1 r2:N.
+  Definition Entry t xs' := startof t xs' = (Addr 100, s).
+  Definition Models := models pil32typctx s.
+  Definition TraceConditions s' := s' R_R1 = r1 /\ s' R_R2 = r2.
+  Definition Init t xs' := Entry t xs' /\ Models.
+
+  Definition Invs (t:trace) :=
+    match t with (Addr a, s)::_ =>
+      match a with
+      | 100 => Some (TraceConditions s)
+      | 124 => Some (True)
+      | _ => None
+      end
+    | _ => None
+    end.
+End Invs.
+
+Definition exit (t:trace) :=
+  match t with (Addr a, s)::_ =>
+    match a with
+      124 => true
+    | _ => false
+  end | _ => false end.
+
+Example addloop_and_beyond s r1 r2: models pil32typctx s ->
+  nextinv Addloop1.addloop (Invs r1 r2 ) exit false ((Addr 100, s)::nil).
+
+  (* At 104 - start of the loop *)
+  Local Ltac step := pil32_step ; try exact I.
+
+  intro.
+  step.
+  (* At 104 - start of the loop *)
+  step.
+  (* At 120 - about to reach postcondition `True` *) step.
+  step. step. step.
+  step.
+  (* At 120 - about to reach postcondition `True` *) step.
+  step. step. step.
+  step.
+  (* At 120 - about to reach postcondition `True` *) step.
+  step. step. step.
+  step.
+  (* At 120 - about to reach postcondition `True` *) step.
+  step. step. step.
+  (* At 120 - about to reach postcondition `True` *) step.
+  (* We loop endlessly because we're searching for the next invariant
+     to prove. After 2^32 iterations of the loop we'll be able to show
+     a contradiction using all the branch conditions, but in Formal Methods
+     we prefer to work smart rather than hard. *)
+Abort.
+End AddloopAndBeyond.
+
+
+
+(** **** Exercise: 1 star, standard, optional (addloop_bookkeeping)
+
+    Modify the invariants and proof for the following addloop to show this version
+    is also correct.  This will demonstrate the need for storing bookkeeping information
+    in loop invariants.  Most of your work should be copy-pasting.*)
+
+Module Addloop'.
+Definition addloop (s:store) (a:addr) : option (N * stmt) :=
+  match a with
+  (* li r3 0x1 *)
+  | 100 => Some(4, Move (R_R3) (Word 1 32))
+  (* :loop *)
+  (* beqz r1 :exit *)
+  | 104 => Some(4, If (BinOp OP_EQ (Var R_R1) (Word 0 32)) (Jmp (Word 120 32)) (Nop))
+  (* sub r1 r1 r3 *)
+  | 108 => Some(4, Move R_R1 (BinOp OP_MINUS (Var R_R1) (Var R_R3)))
+  (* add r2 r2 r3 *)
+  | 112 => Some(4, Move R_R2 (BinOp OP_PLUS  (Var R_R2) (Var R_R3)))
+  (* jmp :loop *)
+  | 116 => Some(4, Jmp (Word 104 32))
+  (* :exit *)
+  (* mov r0 r2 *)
+  | 120 => Some(4, Move R_R0 (Var R_R2))
+  | _ => None
+  end.
+
+Theorem addloop_welltyped : welltyped_prog pil32typctx addloop.
+Proof. Picinae_typecheck. Qed.
+
+Section Invs.
+  (* CHANGE THESE *)
+  Definition Entry := True.
+  Definition Models := True.
+  Definition Init := True.
+
+  Definition postcondition := False.
+
+  Definition Invs (t:trace) := Some (False).
+
+  Definition exit (t:trace) := true.
+
+End Invs.
+
+Theorem addloop_partial_correctness:
+  forall (s:store) t xs' (r1 r2:N) (INIT : Init),
+  satisfies_all addloop Invs exit (xs'::t).
+Proof.
+  (* FILL IN HERE *)
+Admitted.
+End Addloop'.
+
+End Addloop.
+
+(** Exercise:4 stars, standard, optional (sumton)
+
+    Prove the following iterative sum adds up to the closed form expression
+   [(n*(n+1))/2 mod 2^32] when n>1 is given as input to R_R1. *)
+Module SumToN.
+Definition sumton (s:store) (a:addr) : option (N * stmt) :=
+  match a with
+  (* li r3 0x1 *)
+  | 100 => Some(4, Move (R_R3) (Word 1 32))
+  (* li r2 0x0 *)
+  | 104 => Some(4, Move (R_R2) (Word 0 32))
+  (* :loop *)
+  (* blt r1 r3 :exit *)
+  | 108 => Some(4, If (BinOp OP_LT (Var R_R1) (Var R_R3)) (Jmp (Word 124 32)) (Nop))
+  (* add r2 r2 r3 *)
+  | 112 => Some(4, Move R_R2 (BinOp OP_PLUS (Var R_R2) (Var R_R3)))
+  (* add r3 r3 0x1 *)
+  | 116 => Some(4, Move R_R3 (BinOp OP_PLUS (Var R_R3) (Word 1 32)))
+  (* jmp :loop *)
+  | 120 => Some(4, Jmp (Word 108 32))
+  (* :exit *)
+  (* mov r0 r2 *)
+  | 124 => Some(4, Move R_R0 (Var R_R2))
+  (* ret *)
+  | 128 => Some(4, Jmp (Var R_LR))
+  | _ => None
+  end.
+
+Theorem sumton_welltyped : welltyped_prog pil32typctx sumton.
+Proof. Picinae_typecheck. Qed.
+
+Section Invs.
+  (* Change the Init, postcondition, and Invs functions as necessary. *)
+  Variable s : store.
+  Definition Entry t xs' := startof t xs' = (Addr 100, s).
+  Definition Models := models pil32typctx s.
+  Definition Init t xs' n := Entry t xs' /\ Models /\ s R_R1 = n.
+
+  Definition postcondition (s':store) (n:N) := True.
+
+  Definition Invs n (t:trace) := match t with (Addr a, s)::_ =>
+    match a with
+    | 100 => Some (s R_R1 = n)
+    | 116 => Some (True)
+    | 128 => Some (postcondition s n)
+    | _ => None
+    end | _ => None end.
+
+  Definition exit (t:trace) := match t with (Addr 128,_)::_ => true | _=> false end.
+
+End Invs.
+
+Theorem sumton_partial_correctness:
+  forall (s:store) t xs' (n:N) (INIT : Init s t xs' n),
+  satisfies_all sumton (Invs n) exit (xs'::t).
+Proof.
+  Local Ltac step := pil32_step.
+  (* FILL IN HERE *)
+Admitted.
+End SumToN.
+
+(** Exercise:4 stars, standard, optional (factorial)
+
+    Prove the following loop computes the lower 32 bits of the factorial
+    of the value initially in R_R3.*)
+Module Factorial.
+
+Definition factorial (s:store) (a:addr) : option (N * stmt) :=
+  match a with
+    (* li r1 0x1 *)
+  | 100 => Some(4, Move R_R1 (Word 1 32))
+    (* beqz r3 :exit *)
+  | 104 => Some(4, If (BinOp OP_EQ (Var R_R3) (Word 0 32)) (Jmp (Word 140 32)) Nop)
+    (* li r2 0x1 *)
+  | 108 => Some(4, Move R_R2 (Word 1 32))
+    (* nop *)
+  | 112 => Some(4, Nop)
+    (* :loop *)
+    (* beq r2 r3 :loop_done *)
+  | 116 => Some(4, If (BinOp OP_EQ (Var R_R2) (Var R_R3)) (Jmp (Word 136 32)) Nop)
+    (* mul r1 r1 r2 *)
+  | 120 => Some(4, Move R_R1 (BinOp OP_TIMES (Var R_R1) (Var R_R2)))
+    (* add r2 r2 0x1 *)
+  | 124 => Some(4, Move R_R2 (BinOp OP_PLUS (Var R_R2) (Word 1 32)))
+    (* jmp :loop *)
+  | 128 => Some(4, Jmp (Word 116 32))
+    (* nop *)
+  | 132 => Some(4, Nop)
+    (* :loop_done *)
+  | 136 => Some(4, Move R_R1 (BinOp OP_TIMES (Var R_R1) (Var R_R2)))
+    (* :exit *)
+    (* nop *)
+  | 140 => Some(4, Nop)
+  | _ => None
+  end.
+
+Theorem factorial_welltyped : welltyped_prog pil32typctx factorial.
+Proof. Picinae_typecheck. Qed.
+
+Section Invs.
+  (* For this exercise you only need to change the loop invariant in Invs. *)
+  Variable s : store.
+  Definition Entry t xs' := startof t xs' = (Addr 100, s).
+  Definition Models := models pil32typctx s.
+  Definition Init t xs' r3 := Entry t xs' /\ Models /\ s R_R3 = r3.
+
+  Fixpoint natfactorial (n:nat) :=
+    match n with O => 1 | S n' => (N.of_nat n) * (natfactorial n') end.
+  Definition postcondition s' r3 := s' R_R1 = natfactorial (N.to_nat r3) mod 2^32.
+
+  Definition Invs r3 (t:trace) := match t with (Addr a, s)::_ =>
+    match a with
+    | 100 => Some (s R_R3 = r3)
+    | 124 => Some (True)
+    | 140 => Some (postcondition s r3)
+    | _ => None
+    end | _ => None end.
+
+
+  Definition exit (t:trace) := match t with (Addr 140, _)::_ => true | _ => false end.
+
+End Invs.
+
+(** You might find these lemmas helpful in your proofs. *)
+Lemma natfactorial_pred:
+  forall n, natfactorial n * N.of_nat (S n) = natfactorial (S n).
+Proof.
+  induction n.
+  - reflexivity.
+  - unfold natfactorial at 2. rewrite N.mul_comm, N.mul_cancel_l; try lia.
+    rewrite <-IHn, N.mul_comm, N.mul_cancel_l; try lia.
+    reflexivity.
+Qed.
+
+Lemma S_to_nat :
+  forall n, N.to_nat (1+n) = S (N.to_nat n).
+Proof.
+  intros. now rewrite N.add_1_l, N2Nat.inj_succ.
+Qed.
+
+Lemma Nsucc_S :
+  forall n, N.succ n = N.of_nat (S (N.to_nat n)).
+Proof.
+  intros.
+  now rewrite Nat2N.inj_succ, N2Nat.id.
+Qed.
+
+Lemma mod_mono_r :
+  forall x b y, x < y -> x mod b < y.
+Proof.
+  intros. eapply N.le_lt_trans.
+  apply N.Div0.mod_le.
+  assumption.
+Qed.
+
+(** This is the theorem you need to prove. *)
+Theorem factorial_partial_correctness:
+  forall (s:store) t xs' (r3:N) (INIT : Init s t xs' r3),
+  satisfies_all factorial (Invs r3) exit (xs'::t).
+Proof.
+  Local Ltac step := pil32_step.
+  (* FILL IN HERE *)
+Admitted.
+End Factorial.
+
+
+(** **** Exercise:4 stars, standard, recommended (wcscpy_partial_correctness)
+
+    Specify and prove the partial correctness of this simplified wcscpy
+    implementation.  This is the first usage of memory in this tutorial, and not
+    only that, but of memory-writes.  We've placed the invariants at the locations
+    we used to prove this correct and left some of the loop-invariant intact with
+    additional explanation below.
+
+    You'll find many abstractions provided by Picinae are useful for this exercise.
+    Below is a complete list of what we used;  you can find more details about
+    these abstractions in the chapter [AbsAndPracs].
+
+      * [wstrlen] (wrapped up in the [strlen'] definition below)
+      * [wnilfree]
+      * [overlap] and [~ overlap]
+      * mem_region_unchanged
+*)
+Module wcscpy.
+(** r1 - pointer to source wide character string being copied.
+    r0 - pointer to destination *)
+Definition wcscpy (s:store) (a:addr) : option (N * stmt) :=
+  match a with
+  (* 0x00100000: mov r2,#0x0 *)
+  | 1048576 => Some (4, Move R_R2 (Word 0 32))
+
+  (* 0x00100004: ldr r3,[r1, r2, LSL #0x0] *)
+  | 1048580 => Some (4,
+    Move R_R3 (Cast CAST_UNSIGNED 32 (Load (Var V_MEM32)
+      (BinOp OP_PLUS (Var R_R1) (BinOp OP_LSHIFT (Var R_R2) (Word 0 32))) LittleE 4)))
+
+  (* 0x00100008: str r3,[r0, r2, LSL #0x0] *)
+  | 1048584 => Some (4,
+    Move V_MEM32 (Store (Var V_MEM32)
+    (BinOp OP_PLUS (Var R_R0) (BinOp OP_LSHIFT (Var R_R2) (Word 0 32)))
+    (Var R_R3)
+    LittleE 4)
+  )
+
+  (* 0x0010000c: add r2,r2,#0x4 *)
+  | 1048588 => Some (4,
+    Move R_R2 (BinOp OP_PLUS (Var R_R2) (Word 4 32)))
+
+  (* 0x00100010: cbnz r3,0x00100004 *)
+  | 1048592 => Some (4,
+    If (BinOp OP_NEQ (Var R_R3) (Word 0 32)) (
+      Jmp (Word 1048580 32)
+    ) (* else *) (
+      Nop
+    )
+  )
+
+  (* 0x00100014: ret *)
+  | 1048596 => Some (4, Nop)
+
+  | _ => None
+  end.
+
+Theorem wcscpy_welltyped : welltyped_prog pil32typctx wcscpy.
+Proof. Picinae_typecheck. Qed.
+
+Definition strlen' := wstrlen 32 LittleE.
+
+Section Invs.
+  Variable s:store.
+  Variable mem psrc pdest len:N.
+  (* CHANGE THESE *)
+  Definition Entry t xs' := startof t xs' = (Addr 0x00100000, s).
+  Definition Models := models pil32typctx s.
+  (** Replace the [True] in Init with your own initial conditions *)
+  Definition Init t xs' := Entry t xs' /\ Models /\
+    s V_MEM32 = mem /\ s R_R0 = pdest /\ s R_R1 = psrc
+    /\ True.
+
+  (** Replace the [True] in the postcondition with your own initial conditions *)
+  Definition postcondition (s:store) :=
+    exists m, s V_MEM32 = m /\ True.
+
+  Definition Invs (t:trace) := match t with (Addr a, s)::_ =>
+  match a with
+  | 0x00100000 => Some (s V_MEM32 = mem /\ s R_R0 = pdest /\ s R_R1 = psrc
+                        /\ True)
+  (** TODO: Explain the exists m, s V_MEM32 = m clause *)
+  | 0x00100004 => Some (exists m, s V_MEM32 = m
+                        /\ strlen' m psrc len
+                        /\ True)
+  | 0x00100014 => Some (postcondition s)
+  | _ => None end | _ => None end.
+
+  Definition exit (t:trace) := match t with (Addr 0x00100014,_)::_ => true | _ => false end.
+
+End Invs.
+
+Theorem wcscpy_partial_correctness:
+  forall (s:store) t xs' (mem psrc pdest len:N) (INIT : Init s mem psrc pdest t xs'),
+  satisfies_all wcscpy (Invs mem psrc pdest len) exit (xs'::t).
+Proof.
+  Local Ltac step := pil32_step.
+  intros s t xs' mem psrc pdest len (ENTRY & MDL & MEM & LEN & NOV).
+  apply prove_invs.
+
+  (* Base Case *)
+  simpl. rewrite ENTRY. step. repeat (assumption || split).
+
+  (* Inductive Case *)
+  (* Explain the current proof obligation *)
+  intros.
+  unfold Entry in *; erewrite startof_prefix in ENTRY; try eassumption.
+  eapply models_at_invariant; try eassumption. apply wcscpy_welltyped. intro MDL1.
+  clear - PRE MDL1. rename t1 into t; rename s1 into s.
+  destruct_inv 32 PRE.
+Abort.
+End wcscpy.
+
