tutorial/Basics.v
@@ -1,0 +1,713 @@
+(** #<link rel="stylesheet" href="sf.css"># *)
+(** * Motivation *)
+
+(* ################################################################# *)
+(** * Introduction *)
+
+(** This introduction demonstrates a proof of program behaviour,
+    the primary use case of Picinae, and explains how this fits
+    into the reliable software ecosystem
+
+    Predicting software behavior is important.
+
+    Driving on a cliff analogy for software reliability:
+
+      *  Unit/Integration Testing is like opening your eyes
+      *  Runtime exception handling is like guard rails
+      *  Model Checking is like simulation
+      *  Formal Proofs are like total knowledge of all configurations of
+         the universe.  You can safely drive with your eyes closed.
+         Sort of.
+
+
+    The first part of this chapter covers the 3 steps required to
+    start writing proofs about programs for a specific architecture.
+    This includes 1) Architecture Specification, 2) Picinae Module
+    instantiation, and 3) LTac machinery definition. Afterwards we
+    use all of it to show how to prove a property of a simple
+    loop-free program. *)
+
+(* ################################################################# *)
+(** * Setting It Up *)
+
+Require Export Picinae_core.
+Require Export Picinae_theory.
+Require Export Picinae_statics.
+Require Export Picinae_finterp.
+Require Export Picinae_simplifier_v1_1.
+Require Export Picinae_ISA.
+Require Import NArith.
+Require Import Structures.Equalities.
+Open Scope N.
+
+(* ================================================================= *)
+(** ** Architecture Specification *)
+
+(** Before we reason about a program we need to define the architecture
+    this program is for.  This architecture specifies the registers and
+    their sizes,  the different memories and their sizes,  word size,
+    and the default endianness.  This can represent a physical or virtual
+    machine.
+
+    Here we use a minimal architecture specification hand crafted for
+    this demonstration.  We will refer to this architecture as "a64" and
+    "A64" in the code to make it clear what definitions and operations
+    are architecture specific. *)
+
+(** _a64var_ enumerates the registers and memories available in our model.
+
+    Subregisters, like the lower 32-bits of a 64 bit register, are not
+    modeled.  It's easier and safer to change the way a 64-bit register is used in
+    a program to emulate the 32-bit subregister's behavior than it is to
+    model them as two distinct registers and ensure that their values
+    are coherent. *)
+
+Inductive a64var :=
+  | V_MEM
+  | R_R0 | R_R1 | R_R2
+  | F_ZR | F_CY.
+
+(** At this point there is no semantics associated with V_MEM, R_R0, etc.
+    Each one may later be defined as a 1-bit register or a 42-bit register.
+    They are just unique identifiers.
+
+    The function _a64typctx_ is what we use to establish the architectural
+    meanings of the different _a64var_'s.  It takes as input an _a64var_
+    and optionally returns its bitwidth. Please note the unusual representation
+    of memory:
+
+      NB. Memory is just a number represented by the concatenation of all bits.
+          Thus its bitwidth is 8 times the number of addressable bytes.
+*)
+
+Definition a64typctx (id:a64var) : option N :=
+  match id with
+  | V_MEM => Some (8*2^64)
+  | R_R0 | R_R1 | R_R2 => Some (64)
+  | F_ZR | F_CY => Some (1)
+  end.
+
+(* ================================================================= *)
+(** ** Module Instantiation *)
+
+(** Picinae makes extending its powers to
+    new architectures simple. Once we've specified an architecture, which
+    is usually a simple copy-paste-modify operation, we instantiate the
+    core modules with the architecture and we're ready to start writing
+    proofs!
+
+    We'll skip over these details here and discuss them in Chapter X. *)
+
+Module MiniA64VarEq <: MiniDecidableType.
+  Definition t := a64var.
+  Definition eq_dec (v1 v2:a64var) : {v1=v2}+{v1<>v2}.
+    decide equality; apply N.eq_dec.
+  Defined.
+  Arguments eq_dec v1 v2 : simpl never.
+End MiniA64VarEq.
+
+Module A64Arch <: Architecture.
+  Module Var := Make_UDT MiniA64VarEq.
+  Definition var := Var.t.
+  Definition store := var -> N.
+  Definition typctx := var -> option bitwidth.
+  Definition archtyps := a64typctx.
+
+  Definition mem_readable (s:store) (a:addr) := True.
+  Definition mem_writable (s:store) (a:addr) := True.
+End A64Arch.
+
+(* Instantiate the Picinae modules with the arm identifiers above. *)
+Module IL_a64 := PicinaeIL A64Arch.
+Export IL_a64.
+Module Theory_a64 := PicinaeTheory IL_a64.
+Export Theory_a64.
+Module Statics_a64 := PicinaeStatics IL_a64 Theory_a64.
+Export Statics_a64.
+Module FInterp_a64 := PicinaeFInterp IL_a64 Theory_a64 Statics_a64.
+Export FInterp_a64.
+
+Module PSimpl_a64 := Picinae_Simplifier_Base IL_a64.
+Export PSimpl_a64.
+Module PSimpl_a64_v1_1 := Picinae_Simplifier_v1_1 IL_a64 Theory_a64 Statics_a64 FInterp_a64.
+Ltac PSimpl_a64.PSimplifier ::= PSimpl_a64_v1_1.PSimplifier.
+
+Module ISA_a64 := Picinae_ISA IL_a64 PSimpl_a64 Theory_a64 Statics_a64 FInterp_a64.
+Export ISA_a64.
+
+(* Introduce unique aliases for tactics in case user loads multiple architectures. *)
+Tactic Notation "a64_psimpl" uconstr(e) "in" hyp(H) := psimpl_exp_hyp uconstr:(e) H.
+Tactic Notation "a64_psimpl" uconstr(e) := psimpl_exp_goal uconstr:(e).
+Tactic Notation "a64_psimpl" "in" hyp(H) := psimpl_hyp H.
+Tactic Notation "a64_psimpl" := psimpl_goal.
+Ltac step := ISA_step.
+(* ================================================================= *)
+(** ** Ltac Machinery*)
+
+(** Picinae uses a lot of machinery to smooth the process of writing proofs
+    about machine code.  Setting it up is just another short copy-paste-modify
+    task.  We explain the machinery in Chapter X. *)
+
+Ltac simpl_memaccs H ::=
+  try reflexivity.
+Ltac fail_seek ::= idtac.
+
+(* ================================================================= *)
+(** ** A Simple Program Proof *)
+
+(** With the modules and machinery set up we can move on to showing how a simple
+    program proof works.  Picinae programs can be represented in many ways, but each
+    way amounts to a function mapping a store and an address to an IL statement
+    for the symbolic interpreter to execute, plus a number of bytes to step forward
+    if execution control falls through.
+
+    The following program is a hand written example, it adds 1 to the value stored in
+    register 2 ([R_R2]), shifts it left, and stores the result in register 1. The addresses
+    100, 104 and 108 are mapped to the made-up number of bytes the instruction takes up in
+    memory (4 in each case) and a single Picinae IL statement that moves the result of an
+    expression into a register.
+
+   The formal semantics of Picinae IL statements are covered in Chapter X.
+*)
+
+Definition demo_program (_:store) (a:addr) : option (N * stmt) :=
+  match a with
+  | 100 => Some (4, Move (R_R2) (BinOp OP_PLUS (Var R_R2) (Word 1 64)))
+  | 104 => Some (4, Move (R_R2) (BinOp OP_LSHIFT (Var R_R2) (Word 1 64)))
+  | 108 => Some (4, Move (R_R0) (Var R_R2))
+  | _ => None
+  end.
+
+(** We'll also need a proof that this program is well typed. We'll get into what that
+    means and why we need it in the next chapter. *)
+Theorem demo_program_welltyped : welltyped_prog a64typctx demo_program.
+Proof.
+  Picinae_typecheck.
+Qed.
+
+(** Next we'll define a function that maps an _execution trace_ to an _invariant_.
+    Briefly, an execution trace is a list of states that a program has passed through
+    with the current state stored in the head; an invariant is a predicate (alternatively,
+    proposition, property) over traces that we wish to prove.
+
+    Informally, the structure of our proof will look like this...
+
+        For our program p:
+        given a prefix trace t0 that satisfies condition Init, a partial function Invs from
+        traces to predicates, and a function that defines when a trace has "exited"
+        we show that all traces t = t1 ++ t0 that continue t0 either exit or reach a trace
+        for which Invs t is defined, and whenever Invs t is defined it is satisfied.
+
+    The core components are:
+
+        1. Init - a predicate over traces that defines our starting conditions.
+        2. Invs - a partial mapping from traces to a predicate over the input trace.
+        3. Exits - a total mapping from traces to whether they have exited.
+
+    We'll create them in order... *)
+
+Definition Init (t:trace) s xs' (r2:N) :=
+  startof t xs' = (Addr 100, s)
+  /\ models a64typctx s
+  /\ s R_R2 = r2
+  .
+
+(** This _Init_ function states that
+
+      1. the trace starts at address 100 and in state s, and
+      2. the value in register R2 is the natural number r2 of type N (type annotated for clarity).
+
+   Next we'll define the _Invs_ function that specifies the properties of traces that we want
+   to prove.  Coming up with these properties, or _invariants_, is the second hardest part of
+   proving properties of assembly code, right after proving properties of modular arithmetic :) *)
+
+(** To start we'll open a new section so we can define some variables and use them in our definitions
+    without maintaining long parameter lists. Although this isn't very useful in this demonstration
+    we've found that this helps with readability and understandibility in realistic endeavors. *)
+
+Section Invs.
+
+(** We define a variable that represents the initial contents of the R2 register. *)
+
+  Variable r2 : N.
+
+(** We define our postcondition separately for clarity and reusability. We could inline it
+    in our _Invs_ function below but then finding it when developing or auditing code would
+    be more cumbersome.  This way we can also reuse it easily in helper lemmas about the
+    postcondition. *)
+  Definition postcondition (n:N) : Prop := N.even n = true.
+
+
+(** Next we define the _Invs_ partial function that maps traces to the invariants they satisfy.
+    The propositions herein will be the proof obligations we see in our proof about the
+    behavior of this program.
+
+   The trickiest part is that we can't use the values of our store directly as natural
+   numbers in propositions because they have the structure _VaN n b_ for some n and b.
+   Instead we use an existential variable that we bind to _n_ and then use this variable
+   as the value of the register in propositions, e.g. in _even n_ below.
+
+    We've defined the entry point of our program as address 100, so it is helpful to put an
+    invariant there. This will typically be a subset of our initial assumptions, specifically
+    those that tell us about the state of the trace upon entry. If we do not include them
+    then we will lose that information when we destruct the proof into its constituent parts.
+    We'll explain more about that in the next chapter where we look at proofs for more
+    complex programs. *)
+
+  Definition Invs (t:trace) : option Prop :=
+    match t with (Addr a, s)::_ =>
+      match a with
+      | 100 => Some (s R_R2 = r2)
+      | 112 => Some (postcondition (s R_R0))
+      | _ => None
+      end
+    | _ => None end.
+End Invs.
+
+(** Lastly we define the exit points in our programs, a total function from traces to a bool
+    indicating whether the trace is at an exit.  This is used to terminate the proof and signal
+    that traces at this point need not reach and satisfy another invariant.
+
+    We set address 112 as our only exit point, this is the address following the last.  If we
+    set it as the final instruction then that instruction will not execute. *)
+Definition exits (t:trace) : bool :=
+  match t with (Addr a, _)::_ =>
+    match a with
+      112 => true
+    | _ => false
+    end
+  | _ => false
+  end.
+
+(** Now that we've defined 1) the initial conditions of traces we're reasoning about, 2) the
+    properties we will prove they satisfy and 3) the exit points, we are finally ready
+    to write the proof! *)
+
+Theorem prog_partial_correctness :
+  forall s t xs' r2 (INIT: Init t s xs' r2),
+    satisfies_all demo_program (Invs r2) exits (xs'::t).
+Proof.
+  intros. destruct INIT as (ENTRY & MDL & R2).
+  apply prove_invs.
+
+  (* Base Case *)
+  simpl. rewrite ENTRY. step. assumption.
+
+  (* Inductive Case *)
+  intros.
+  erewrite startof_prefix in ENTRY; try eassumption.
+  eapply models_at_invariant; try eassumption. apply demo_program_welltyped. intro MDL1.
+  clear - PRE MDL1. rename t1 into t; rename s1 into s.
+  destruct_inv 64 PRE.
+
+  step. step. step.
+
+  (* Postcondition *)
+  rewrite update_updated.
+  destruct (1 + r2) eqn:Eq.
+    reflexivity.
+    apply mp2_even. all: easy.
+Qed.
+
+(** **** Exercise:1 stars, recommended, swap_register_addition
+
+    In this exercise you will specify and prove that this short program for our
+    hypothetical architecture swaps the values of its R0 and R1 registers. *)
+Module swap_register_addition.
+
+(** This is the (handwritten) program definition.  We continue with the pretense
+    that each instruction is 4 bytes long.  It implements the typical algorithm
+    to swap the values of two register/variables using addition.  Does it work
+    in our modular arithmetic setting?  You will prove that it does. *)
+Definition swap_regs (s:store) (a:addr) : option (N * stmt) :=
+  match a with
+  | 100 => Some(4, Move R_R0 (BinOp OP_PLUS  (Var R_R0) (Var R_R1)))
+  | 104 => Some(4, Move R_R1 (BinOp OP_MINUS (Var R_R0) (Var R_R1)))
+  | 108 => Some(4, Move R_R0 (BinOp OP_MINUS (Var R_R0) (Var R_R1)))
+  | 112 => Some(4, Nop)
+  | _ => None
+  end.
+
+(** The welltyped program theorem checks that the handwritten program has no
+    obvious flaws, e.g., storing 64-bit values in 32-bit registers, and is used
+    in the proof to enable sound automation.  *)
+Theorem swap_regs_welltyped : welltyped_prog a64typctx swap_regs.
+Proof. Picinae_typecheck. Qed.
+
+
+Section Invs.
+
+  (** These variables represent the initial value of the store, [R0] and [R1]
+      respectively. *)
+  Variable s:store.
+  Variable r0 r1:N.
+
+  (** In these tutorials we define the "entry" and "models" propositions
+      independently to highlight their ubiquity.  Above these are the
+      [startof t xs' = (Addr 100, s)] and [models a64typctx s] clauses of the
+      [Init] proposition. Conveniently, the same propositions fit here as well. *)
+  Definition Entry t xs' := startof t xs' = (Addr 100, s).
+  Definition Models := models a64typctx s.
+
+  (** Replace the [True] with two clauses binding [R0] and [R1] in the initial
+      store [s] to the two variables [r0] and [r1] we declared above. *)
+  Definition Init t xs' := Entry t xs' /\ Models /\ (* True *) s R_R0 = r0 /\ s R_R1 = r1.
+
+  (** Replace the [False] with a proposition stating that the values of registers
+      [R0] and [R1] in the final store have been swapped.  Note that the [s] here
+      is a parameter name that shadows the [s] variable in this section. *)
+  Definition postcondition (s:store) := (* False *) s R_R0 = r1 /\ s R_R1 = r0.
+
+  (** Note that the [s] in the match pattern below shadows the [s] variable in
+      this section.  We don't need it here because we've used it above.  If we
+      have a proof where we need to refer to the initial store in the invariants
+      then we would change one of two names. *)
+  Definition Invs (t:trace) := match t with (Addr a, s)::_ =>
+    match a with
+    (** This is the starting invariant.  Typically it is the same as the definition
+        of [Init] minus the [Entry] and [Models] clauses, so add the clauses
+        you added there here. *)
+    | 100 => Some (True)
+    (** This is the postcondition invariant.  We place it at the program's exit
+        address.  In this simple example this is 112, the [Nop] instruction.
+        We will need to prove this invariant holds _before_ executing the
+        instruction, [Nop] in this case. *)
+    | 112 => Some ( postcondition s)
+    (** No other addresses nor exit conditions (e.g., exceptions) have invariants
+        that we need to prove, so we mark them with [None]. *)
+    | _ => None end | _ => None end.
+
+  (** Finally, the program exits for any trace that reaches address 112, so replace
+     the constant [true] with the corresponding expression. *)
+  (* Definition exits (t:trace) := true. *)
+  Definition exits (t:trace) := match t with (Addr 112, _)::_ => true | _ => false end.
+
+End Invs.
+
+Theorem swap_regs_partial_correctness:
+  forall (s:store) t xs' (r0 r1:N) (INIT : Init s r0 r1 t xs'),
+  satisfies_all swap_regs (Invs r0 r1) exits (xs'::t).
+Proof.
+  intros. destruct INIT as (ENTRY & MDL & R0 & R1).
+  apply prove_invs.
+
+  (* Base Case *)
+  simpl. rewrite ENTRY. step.
+  (* FILL IN HERE (replace the admit.)*)
+  admit.
+
+  (* Inductive Case *)
+  intros.
+  unfold Entry in *; erewrite startof_prefix in ENTRY; try eassumption.
+  eapply models_at_invariant; try eassumption. apply swap_regs_welltyped. intro MDL1.
+  clear - PRE MDL1. rename t1 into t; rename s1 into s.
+  destruct_inv 64 PRE.
+
+  (* FILL IN HERE *)
+Admitted.
+End swap_register_addition.
+
+
+(** **** Exercise:1 stars, optional, swap_register_xor
+
+    This exercise is a repeat of register swapping, this time using exclusive-or
+    and with less hand-holding. *)
+Module swap_register_xor.
+Definition swap_regs (s:store) (a:addr) : option (N * stmt) :=
+  match a with
+  | 300 => Some(4, Move R_R0 (BinOp OP_XOR (Var R_R0) (Var R_R1)))
+  | 304 => Some(4, Move R_R1 (BinOp OP_XOR (Var R_R0) (Var R_R1)))
+  | 308 => Some(4, Move R_R0 (BinOp OP_XOR (Var R_R0) (Var R_R1)))
+  | 312 => Some(4, Nop)
+  | _ => None
+  end.
+
+(** The welltyped program theorem checks that the handwritten program has no
+    obvious flaws, e.g., storing 64-bit values in 32-bit registers, and is used
+    in the proof to enable sound automation.  *)
+Theorem swap_regs_welltyped : welltyped_prog a64typctx swap_regs.
+Proof. Picinae_typecheck. Qed.
+
+
+Section Invs.
+
+  Variable s:store.
+  Variable r0 r1:N.
+
+  Definition Entry t xs' := startof t xs' = (Addr 300, s).
+  Definition Models := models a64typctx s.
+  Definition Init t xs' := Entry t xs' /\ Models /\ True (* <- replace this True *).
+
+  Definition postcondition (s:store) := False (* <- replace this False *).
+
+  Definition Invs (t:trace) := match t with (Addr a, s)::_ =>
+    match a with
+    | 300 => Some (True)
+    | 312 => Some (postcondition s)
+    | _ => None end | _ => None end.
+
+  Definition exit (t:trace) := true.
+
+End Invs.
+
+(* Make whatever changes you need to the theorem specification to prove it. *)
+Theorem swap_regs_partial_correctness:
+  forall (s:store) t xs' (INIT : Init s t xs'),
+  satisfies_all swap_regs (Invs) exits (xs'::t).
+Proof.
+  intros. destruct INIT as (ENTRY & MDL & T).
+  apply prove_invs.
+
+  (* Base Case *)
+  simpl. rewrite ENTRY. step.
+  (* FILL IN HERE (replace the admit.)*)
+  admit.
+
+  (* Inductive Case *)
+  intros.
+  unfold Entry in *; erewrite startof_prefix in ENTRY; try eassumption.
+  eapply models_at_invariant; try eassumption. apply swap_regs_welltyped. intro MDL1.
+  clear - PRE MDL1. rename t1 into t; rename s1 into s.
+  destruct_inv 64 PRE.
+
+  (* FILL IN HERE *)
+Admitted.
+End swap_register_xor.
+
+(* begin details *)
+Declare Scope pil_stmt_scope.
+Open Scope pil_stmt_scope.
+Notation " s1 $; s2 " := (Seq s1 s2) (at level 75, right associativity) : pil_stmt_scope.
+(* end details *)
+
+(** **** Exercise:3 stars, optional, tolower
+
+    The following is a version of to_lower compiled for the Armv8 architecture,
+    minimmally modified for this chapter.  This gives a better perspective
+    of what real code looks like. *)
+
+Module tolower.
+Definition tolower (s:store) (a:addr) : option (N * stmt) :=
+  match a with
+  (* 0x00200000: sub w1,w0,#0x41 *)
+  | 2097152 => Some (4,
+    Move R_R1 (Cast CAST_UNSIGNED 64 (BinOp OP_MINUS (Extract 31 0 (Var R_R0)) (Word 65 32))))
+
+  (* 0x00200004: cmp w1,#0x19 *)
+  | 2097156 => Some (4,
+    Move F_CY (BinOp OP_LE (Word 25 32) (Extract 31 0 (Var R_R1))) $;
+    Move F_ZR (BinOp OP_EQ (BinOp OP_MINUS (Extract 31 0 (Var R_R1)) (Word 25 32)) (Word 0 32)))
+
+  (* 0x00200008: b.hi 0x00200010 *)
+  | 2097160 => Some (4,
+    If (Cast CAST_LOW 1 (BinOp OP_AND (Var F_CY) (UnOp OP_NOT (Var F_ZR)))) (
+      Jmp (Word 2097168 64)
+    ) (* else *) (
+      Nop
+    ))
+
+  (* 0x0020000c: orr w0,w0,#0x20 *)
+  | 2097164 => Some (4,
+    Move R_R0 (Cast CAST_UNSIGNED 64 (BinOp OP_OR (Extract 31 0 (Var R_R0)) (Word 32 32))))
+
+  (* 0x00200010: ret *)
+  | 2097168 => Some (4,
+    Nop)
+
+  | _ => None
+  end.
+
+Theorem tolower_welltyped : welltyped_prog a64typctx tolower.
+Proof. Picinae_typecheck. Qed.
+
+
+Section Invs.
+
+  Variable s:store.
+
+  Definition Entry (t:trace) (xs':exit*store) := startof t xs' = (Addr 0x00200000, s).
+  Definition Models := models a64typctx s.
+  Definition Init t xs' := Entry t xs' /\ Models /\ True.
+
+  Definition postcondition (s:store) := False.
+
+  Definition Invs (t:trace) := match t with (Addr a, s)::_ =>
+    match a with
+    | 0x00200000 => Some (True)
+    | 0x00200010 => Some (postcondition s)
+    | _ => None end | _ => None end.
+
+  Definition exit (t:trace) := match t with (Addr 0x00200010, _)::_ => true | _ => false end.
+
+End Invs.
+
+Theorem tolower_partial_correctness:
+  forall (s:store) t xs' (INIT : Init s t xs'),
+  satisfies_all tolower (Invs) exit (xs'::t).
+Proof.
+  intros. destruct INIT as (ENTRY & MDL & W0).
+  apply prove_invs.
+
+  (* Base Case *)
+  simpl. rewrite ENTRY. step.
+  (* FILL IN HERE (replace the admit.)*)
+  admit.
+
+  (* Inductive Case *)
+  intros.
+  unfold Entry in *; erewrite startof_prefix in ENTRY; try eassumption.
+  eapply models_at_invariant; try eassumption. apply tolower_welltyped. intro MDL1.
+  clear - PRE MDL1. rename t1 into t; rename s1 into s.
+  destruct_inv 64 PRE.
+
+  repeat step.
+Admitted.
+End tolower.
+
+
+(** **** Exercise:4 stars, optional, toupper
+
+    The following is a version of toupper compiled for the Armv8 architecture,
+    minimmally modified for this chapter.  This gives a better perspective
+    of what real code looks like. *)
+
+
+Module toupper.
+Definition toupper (s:store) (a:addr) : option (N * stmt) :=
+  match a with
+  (* 0x00100000: sub w1,w0,#0x61 *)
+  | 1048576 => Some (4,
+    Move R_R1 (Cast CAST_UNSIGNED 64 (BinOp OP_MINUS (Extract 31 0 (Var R_R0)) (Word 97 32))))
+
+  (* 0x00100004: cmp w1,#0x19 *)
+  | 1048580 => Some (4,
+    Move F_ZR (BinOp OP_EQ (BinOp OP_MINUS (Extract 31 0 (Var R_R1)) (Word 25 32)) (Word 0 32)) $;
+    Move F_CY (BinOp OP_LE (Word 25 32) (Extract 31 0 (Var R_R1))))
+
+  (* 0x00100008: b.hi 0x00100014 *)
+  | 1048584 => Some (4,
+    If (Cast CAST_LOW 1 (BinOp OP_AND (Var F_CY) (UnOp OP_NOT (Var F_ZR)))) (
+      Jmp (Word 1048596 64)
+    ) (* else *) (
+      Nop
+    )
+  )
+
+  (* 0x0010000c: mov w1,#0x5f *)
+  | 1048588 => Some (4,
+    Move R_R1 (Word 95 64))
+
+  (* 0x00100010: and w0,w0,w1 *)
+  | 1048592 => Some (4,
+    Move R_R0 (Cast CAST_UNSIGNED 64 (BinOp OP_AND (Extract 31 0 (Var R_R0)) (Extract 31 0 (Var R_R1)))))
+
+  (* 0x00100014: ret *)
+  | 1048596 => Some (4,
+    Nop)
+  | _ => None
+  end.
+
+Theorem toupper_welltyped : welltyped_prog a64typctx toupper.
+Proof. Picinae_typecheck. Qed.
+
+
+Section Invs.
+
+  Variable s:store.
+  Variable w0:N.
+
+  Definition Entry (t:trace) (xs':exit*store) := (* True *) startof t xs' = (Addr 0x00100000, s).
+  Definition Models := models a64typctx s.
+  Definition Init t xs' := Entry t xs' /\ Models /\ (* True *) s R_R0 = w0.
+
+  Definition postcondition (s:store) := if andb (97 <=? w0) (w0 <=? 122) then s R_R0 = w0 - 32 else s R_R0 = w0.
+
+  Definition Invs (t:trace) := match t with (Addr a, s)::_ =>
+    match a with
+      (* | 100 => Some (True) *)
+    | 0x00100000 => Some (s R_R0 = w0)
+    | 0x00100014 => Some (postcondition s)
+    | _ => None end | _ => None end.
+
+  (* Definition exit (t:trace) := true. *)
+  Definition exit (t:trace) := match t with (Addr 0x00100014, _)::_ => true | _ => false end.
+
+End Invs.
+
+Theorem toupper_partial_correctness:
+  forall (s:store) t xs' (w0:N) (INIT : Init s w0 t xs'),
+  satisfies_all toupper (Invs w0) exit (xs'::t).
+Proof.
+  intros. destruct INIT as (ENTRY & MDL & W0).
+  apply prove_invs.
+
+  (* Base Case *)
+  simpl. rewrite ENTRY. step.
+  (* FILL IN HERE (replace the admit.)*)
+  admit.
+
+  (* Inductive Case *)
+  intros.
+  unfold Entry in *; erewrite startof_prefix in ENTRY; try eassumption.
+  eapply models_at_invariant; try eassumption. apply toupper_welltyped. intro MDL1.
+  clear - PRE MDL1. rename t1 into t; rename s1 into s.
+  destruct_inv 64 PRE.
+
+  repeat step.
+Admitted.
+End toupper.
+
+(** To close off this chapter we hone in on Picinae's abstract execution with an example
+    that isolates it from proofs of program properties.
+
+    After some initial setup we see how Picinae uses Coq as an abstract execution engine.
+    Each [step] call executes one machine instruction at the current address and replaces
+    the goal with each possible result of the instruction call.
+
+    We'll cover what's going on with the proof, including the mystery of xs', in the following chapter.
+    This is enough to show off the most basic user experience of proving properties of programs with
+    Picinae.
+
+    Before we wrap up we'd like to impress upon you Picinae's abstract execution ability with
+    one more example.  In the program below, the instruction at address 0 jumps to 1 of 6
+    possible destinations or falls through depending on a sequence of condition checks. *)
+
+Definition multijump (s:store) (a:addr) : option (N * stmt) :=
+  match a with
+  | 0 => Some(1, If (BinOp OP_EQ (Var R_R0) (Word 0 64)) (Jmp (Word 1 64))
+                 (If (BinOp OP_EQ (Var R_R0) (Word 1 64)) (Jmp (Word 2 64))
+                 (If (BinOp OP_EQ (Var R_R0) (Word 2 64)) (Jmp (Word 3 64))
+                 (If (BinOp OP_EQ (Var R_R0) (Word 3 64)) (Jmp (Word 4 64))
+                 (If (BinOp OP_EQ (Var R_R0) (Word 4 64)) (Jmp (Word 5 64))
+                 (If (BinOp OP_EQ (Var R_R0) (Word 5 64)) (Jmp (Word 6 64)) (Nop)))))))
+  | 1 => Some(1, Exn 1)
+  | 2 => Some(1, Exn 2)
+  | 3 => Some(1, Exn 3)
+  | 4 => Some(1, Exn 4)
+  | 5 => Some(1, Exn 5)
+  | 6 => Some(1, Exn 6)
+  | _ => None
+  end.
+
+(** Let's set up an environment where we start at address 0. *)
+
+Example jumpy s : nextinv multijump (fun _ => None) (fun _ => false) false ((Addr 0, s)::nil).
+
+(** Now we take a step. *)
+
+step.
+
+(** Wow!  Look at all of those goals!  Picinae interpreted the instruction and generated a list
+    of 7 subgoals corresponding to all possible evaluations and exits, including the fall through,
+    and updated the contexts of each with a Branch Condition (BC) that shows the conditions necessary
+    for this trace.
+
+    If we take a close look we see that the goal at the bottom (subgoal 7) is exactly the same as the goal
+    at the top (subgoal 1).  By moving the subgoals around to inspect it we can see all the branch
+    conditions that were necessary to hold for the control to fall through.
+ *)
+all:cycle -1.
+
+(** Now that's exciting. *)
+
+Abort.
